

## Section 7.3 Trigonometric Substitution

### Background

Last class, we reviewed some important trigonometric identities and used them to solve tricky trigonometric integrals. Today we use those identities to solve integrals involving **square roots and polynomials** via **trigonometric substitution**.

### The Set-Up: When Trig Sub Helps

Trig substitution is designed for integrals containing expressions like:

$$\sqrt{a^2 - x^2}, \quad \sqrt{a^2 + x^2}, \quad \sqrt{x^2 - a^2}, \quad \text{where } a \text{ is a constant}$$

The goal is to choose a substitution that turns the square root into a simple trig expression using a Pythagorean identity.

### Core Identities (Pythagorean)

- $\sin^2 \theta + \cos^2 \theta = 1$
- $1 + \tan^2 \theta = \sec^2 \theta$
- $\sec^2 \theta - 1 = \tan^2 \theta$

### Trig Substitution Table

Expression	Substitution	Identity Used
$\sqrt{a^2 - x^2}$	$x = a \sin \theta$	$1 - \sin^2 \theta = \cos^2 \theta$
$\sqrt{a^2 + x^2}$	$x = a \tan \theta$	$1 + \tan^2 \theta = \sec^2 \theta$
$\sqrt{x^2 - a^2}$	$x = a \sec \theta$	$\sec^2 \theta - 1 = \tan^2 \theta$

## Standard Workflow (Checklist)

For each trig substitution integral:

**Step 1: Identify the root form** ( $\sqrt{a^2 - x^2}$ ,  $\sqrt{a^2 + x^2}$ , or  $\sqrt{x^2 - a^2}$ ) and pick the matching substitution.

**Step 2: Differentiate** the substitution to rewrite  $dx$  in terms of  $d\theta$ .

**Step 3: Rewrite the entire integrand** in terms of  $\theta$  (including the square root).

**Step 4: Simplify** using trig identities; integrate with trig techniques.

**Step 5: Draw a reference triangle** to convert back to  $x$  (or use inverse trig carefully).

**Step 6: Back-substitute** and include  $+C$ .

## Triangle Back-Sub Templates

Use these to return from  $\theta$  to  $x$ .

**If  $x = a \sin \theta$**

Then  $\sin \theta = \frac{x}{a}$ , so draw a right triangle with:

$$\text{opposite} = x, \quad \text{hypotenuse} = a, \quad \text{adjacent} = \sqrt{a^2 - x^2}.$$

$$\text{Common outputs: } \cos \theta = \frac{\sqrt{a^2 - x^2}}{a}.$$

**If  $x = a \tan \theta$**

Then  $\tan \theta = \frac{x}{a}$ , so draw a right triangle with:

$$\text{opposite} = x, \quad \text{adjacent} = a, \quad \text{hypotenuse} = \sqrt{a^2 + x^2}.$$

$$\text{Common outputs: } \sec \theta = \frac{\sqrt{a^2 + x^2}}{a}.$$

**If  $x = a \sec \theta$**

Then  $\sec \theta = \frac{x}{a}$ , so  $\cos \theta = \frac{a}{x}$  and draw a right triangle with:

$$\text{adjacent} = a, \quad \text{hypotenuse} = x, \quad \text{opposite} = \sqrt{x^2 - a^2}.$$

$$\text{Common outputs: } \tan \theta = \frac{\sqrt{x^2 - a^2}}{a}.$$

(1)  $\int \sqrt{1-x^2} \, dx$

(2)  $\int \sqrt{1+x^2} \, dx$

(3)  $\int \frac{1}{x^2\sqrt{x^2+2}} dx$

(4)  $\int \frac{1}{(4x^2 + 9)^2} dx$

(5)  $\int x^3 \sqrt{1 + 4x^2} \, dx$